spec/machine/ARM/MachineOps.thy
@@ -346,9 +346,9 @@ where
     is_masked \<leftarrow> gets $ irq_masks;
     modify (\<lambda>s. s \<lparr> irq_state := irq_state s + 1 \<rparr>);
     active_irq \<leftarrow> gets $ irq_oracle \<circ> irq_state;
-    if is_masked active_irq \<or> active_irq = 0x3FF \<or> (in_kernel \<and> active_irq \<in> non_kernel_IRQs)
+    if is_masked active_irq \<or> (in_kernel \<and> active_irq \<in> non_kernel_IRQs)
     then return None
-    else return ((Some active_irq) :: irq option)
+    else return (Some active_irq)
   od"
 
 definition
